Prove head thm for new_type (which is now: call_new_type)

candle/prover/candle_kernel_valsScript.sml
@@ -31,7 +31,7 @@ Definition kernel_funs_def:
 
     types_v;
     get_type_arity_v;
-    new_type_v;
+    call_new_type_v;
     mk_type_v;
     mk_vartype_v;
     dest_type_v;
@@ -239,8 +239,8 @@ Definition STRING_TYPE_HEAD_def:
   STRING_TYPE_HEAD v ⇔ ∃s. STRING_TYPE s v
 End
 
-Definition NUM_HEAD_def:
-  NUM_HEAD v ⇔ ∃n. NUM n v
+Definition INT_HEAD_def:
+  INT_HEAD v ⇔ ∃n. INT n v
 End
 
 (* -------------------------------------------------------------------------
@@ -948,99 +948,6 @@ Proof
   \\ fs [] \\ strip_tac \\ gvs [] \\ metis_tac []
 QED
 
-Theorem vsubst_v_head:
-  do_partial_app vsubst_v v = SOME g ∧
-  do_opapp [g; w] = SOME (env, exp) ∧
-  evaluate ^s env [exp] = (s', res) ⇒
-    ^safe_error_goal ∨
-    LIST_TYPE_HEAD (PAIR_TYPE_HEAD TERM_TYPE_HEAD TERM_TYPE_HEAD) v ∧
-    TERM_TYPE_HEAD w
-Proof
-  rewrite_tac [vsubst_v_def]
-  \\ qmatch_goalsub_rename_tac ‘Let NONE _ (Let NONE _ ee)’
-  \\ strip_tac
-  \\ gvs [do_partial_app_def,do_opapp_def]
-  \\ pop_assum mp_tac
-  \\ ntac 5 (simp [Once evaluate_def])
-  \\ CONV_TAC (DEPTH_CONV ml_progLib.nsLookup_conv) \\ simp []
-  \\ qspecl_then [‘v’,‘s’] strip_assume_tac check_tm_tm_head
-  \\ fs [] \\ rw [] \\ fs [namespaceTheory.nsOptBind_def] \\ rewrite_tac [same_clock_exists]
-  \\ drule_then (qspec_then ‘w’ mp_tac) evaluate_tm_check
-  \\ CONV_TAC (DEPTH_CONV ml_progLib.nsLookup_conv) \\ simp []
-  \\ gvs [ml_progTheory.nsLookup_Short_def,pmatch_def,
-          ml_progTheory.nsLookup_nsBind_compute,ml_progTheory.merge_env_def]
-  \\ CONV_TAC (DEPTH_CONV ml_progLib.nsLookup_conv) \\ simp []
-  \\ strip_tac \\ fs [same_clock_exists]
-QED
-
-Theorem inst_v_head:
-  do_partial_app inst_v v = SOME g ∧
-  do_opapp [g; w] = SOME (env, exp) ∧
-  evaluate ^s env [exp] = (s', res) ⇒
-    ^safe_error_goal ∨
-    LIST_TYPE_HEAD (PAIR_TYPE_HEAD TYPE_TYPE_HEAD TYPE_TYPE_HEAD) v ∧
-    TERM_TYPE_HEAD w
-Proof
-  rewrite_tac [inst_v_def]
-  \\ qmatch_goalsub_rename_tac ‘Let NONE _ (Let NONE _ ee)’
-  \\ strip_tac
-  \\ gvs [do_partial_app_def,do_opapp_def]
-  \\ pop_assum mp_tac
-  \\ ntac 5 (simp [Once evaluate_def])
-  \\ CONV_TAC (DEPTH_CONV ml_progLib.nsLookup_conv) \\ simp []
-  \\ qspecl_then [‘v’,‘s’] strip_assume_tac check_ty_ty_head
-  \\ fs [] \\ rw [] \\ fs [namespaceTheory.nsOptBind_def] \\ rewrite_tac [same_clock_exists]
-  \\ drule_then (qspec_then ‘w’ mp_tac) evaluate_tm_check
-  \\ CONV_TAC (DEPTH_CONV ml_progLib.nsLookup_conv) \\ simp []
-  \\ gvs [ml_progTheory.nsLookup_Short_def,pmatch_def,
-          ml_progTheory.nsLookup_nsBind_compute,ml_progTheory.merge_env_def]
-  \\ CONV_TAC (DEPTH_CONV ml_progLib.nsLookup_conv) \\ simp []
-  \\ strip_tac \\ fs [same_clock_exists]
-QED
-
-Theorem call_variant_v_head:
-  do_partial_app call_variant_v v = SOME g ∧
-  do_opapp [g; w] = SOME (env, exp) ∧
-  evaluate ^s env [exp] = (s', res) ⇒
-    ^safe_error_goal ∨
-    LIST_TYPE_HEAD TERM_TYPE_HEAD v ∧
-    TERM_TYPE_HEAD w
-Proof
-  rewrite_tac [call_variant_v_def]
-  \\ qmatch_goalsub_rename_tac ‘Let NONE _ (Let NONE _ ee)’
-  \\ strip_tac
-  \\ gvs [do_partial_app_def,do_opapp_def]
-  \\ pop_assum mp_tac
-  \\ ntac 5 (simp [Once evaluate_def])
-  \\ CONV_TAC (DEPTH_CONV ml_progLib.nsLookup_conv) \\ simp []
-  \\ qspecl_then [‘v’,‘s’] strip_assume_tac check_tm_head
-  \\ fs [] \\ rw [] \\ fs [namespaceTheory.nsOptBind_def] \\ rewrite_tac [same_clock_exists]
-  \\ drule_then (qspec_then ‘w’ mp_tac) evaluate_tm_check
-  \\ CONV_TAC (DEPTH_CONV ml_progLib.nsLookup_conv) \\ simp []
-  \\ gvs [ml_progTheory.nsLookup_Short_def,pmatch_def,
-          ml_progTheory.nsLookup_nsBind_compute,ml_progTheory.merge_env_def]
-  \\ CONV_TAC (DEPTH_CONV ml_progLib.nsLookup_conv) \\ simp []
-  \\ strip_tac \\ fs [same_clock_exists]
-QED
-
-Theorem beta_v_head:
-  do_opapp [beta_v; v] = SOME (env, exp) ∧
-  evaluate ^s env [exp] = (s', res) ⇒
-    ^safe_error_goal ∨
-    TERM_TYPE_HEAD v
-Proof
-  rewrite_tac [beta_v_def]
-  \\ qmatch_goalsub_rename_tac ‘Let NONE _ ee’
-  \\ strip_tac
-  \\ gvs [do_partial_app_def,do_opapp_def]
-  \\ drule_then (qspec_then ‘v’ mp_tac) evaluate_tm_check
-  \\ CONV_TAC (DEPTH_CONV ml_progLib.nsLookup_conv) \\ simp []
-  \\ gvs [ml_progTheory.nsLookup_Short_def,pmatch_def,
-          ml_progTheory.nsLookup_nsBind_compute,ml_progTheory.merge_env_def]
-  \\ CONV_TAC (DEPTH_CONV ml_progLib.nsLookup_conv) \\ simp []
-  \\ strip_tac \\ fs [same_clock_exists]
-QED
-
 Theorem types_v_head:
   do_opapp [types_v; v] = SOME (env, exp) ∧
   evaluate ^s env [exp] = (s', res) ⇒
@@ -1094,7 +1001,28 @@ Proof
   \\ fs[CaseEqs["v","option","prod","lit"]] \\ gvs[same_clock_exists]
 QED
 
-val one_arg_tac =
+Theorem call_new_type_v_head:
+  do_opapp [call_new_type_v; v] = SOME (env, exp) ∧
+  evaluate ^s env [exp] = (s', res) ⇒
+    ^safe_error_goal ∨
+    PAIR_TYPE_HEAD STRING_TYPE_HEAD INT_HEAD v
+Proof
+  rewrite_tac[kernel_funs_v_def]
+  \\ rewrite_tac [do_partial_app_clos,do_opapp_clos]
+  \\ rpt strip_tac \\ rveq \\ fs []
+  \\ rpt (
+    (dxrule evaluate_str_check ORELSE dxrule evaluate_mat_pair)
+    \\ simp [ml_progTheory.nsLookup_nsBind_compute]
+    \\ CONV_TAC (DEPTH_CONV ml_progLib.nsLookup_conv) \\ simp []
+    \\ rpt strip_tac \\ simp [same_clock_exists])
+  \\ fs [PAIR_TYPE_HEAD_def,PAIR_TYPE_def]
+  \\ pop_assum mp_tac
+  \\ ntac 5 (simp [Once evaluate_def,do_app_def])
+  \\ strip_tac \\ gvs [AllCaseEqs(),same_clock_exists]
+  \\ fs [INT_HEAD_def,INT_def]
+QED
+
+val prove_head_tac =
   rewrite_tac[kernel_funs_v_def]
   \\ TRY (rename [‘Let (SOME xx) yy zz’])
   \\ rewrite_tac [do_partial_app_clos,do_opapp_clos]
@@ -1116,324 +1044,24 @@ val one_arg_tac =
     \\ rpt strip_tac \\ simp [same_clock_exists])
   \\ fs [PAIR_TYPE_HEAD_def,PAIR_TYPE_def];
 
-Theorem dest_type_v_head:
-  do_opapp [dest_type_v; v] = SOME (env, exp) ∧
-  evaluate ^s env [exp] = (s', res) ⇒
-    ^safe_error_goal ∨
-    TYPE_TYPE_HEAD v
-Proof
-  one_arg_tac
-QED
-
-Theorem is_type_v_head:
-  do_opapp [is_type_v; v] = SOME (env, exp) ∧
-  evaluate ^s env [exp] = (s', res) ⇒
-    ^safe_error_goal ∨
-    TYPE_TYPE_HEAD v
-Proof
-  one_arg_tac
-QED
-
-Theorem is_vartype_v_head:
-  do_opapp [is_vartype_v; v] = SOME (env, exp) ∧
-  evaluate ^s env [exp] = (s', res) ⇒
-    ^safe_error_goal ∨
-    TYPE_TYPE_HEAD v
-Proof
-  one_arg_tac
-QED
-
-Theorem is_var_v_head:
-  do_opapp [is_var_v; v] = SOME (env, exp) ∧
+Theorem beta_v_head:
+  do_opapp [beta_v; v] = SOME (env, exp) ∧
   evaluate ^s env [exp] = (s', res) ⇒
     ^safe_error_goal ∨
     TERM_TYPE_HEAD v
 Proof
-  one_arg_tac
+  prove_head_tac
 QED
 
-Theorem is_const_v_head:
-  do_opapp [is_const_v; v] = SOME (env, exp) ∧
-  evaluate ^s env [exp] = (s', res) ⇒
-    ^safe_error_goal ∨
-    TERM_TYPE_HEAD v
-Proof
-  one_arg_tac
-QED
-
-Theorem is_abs_v_head:
-  do_opapp [is_abs_v; v] = SOME (env, exp) ∧
-  evaluate ^s env [exp] = (s', res) ⇒
-    ^safe_error_goal ∨
-    TERM_TYPE_HEAD v
-Proof
-  one_arg_tac
-QED
-
-Theorem is_comb_v_head:
-  do_opapp [is_comb_v; v] = SOME (env, exp) ∧
-  evaluate ^s env [exp] = (s', res) ⇒
-    ^safe_error_goal ∨
-    TERM_TYPE_HEAD v
-Proof
-  one_arg_tac
-QED
-
-Theorem rand_v_head:
-  do_opapp [rand_v; v] = SOME (env, exp) ∧
-  evaluate ^s env [exp] = (s', res) ⇒
-    ^safe_error_goal ∨
-    TERM_TYPE_HEAD v
-Proof
-  one_arg_tac
-QED
-
-Theorem rator_v_head:
-  do_opapp [rator_v; v] = SOME (env, exp) ∧
-  evaluate ^s env [exp] = (s', res) ⇒
-    ^safe_error_goal ∨
-    TERM_TYPE_HEAD v
-Proof
-  one_arg_tac
-QED
-
-Theorem dest_var_v_head:
-  do_opapp [dest_var_v; v] = SOME (env, exp) ∧
-  evaluate ^s env [exp] = (s', res) ⇒
-    ^safe_error_goal ∨
-    TERM_TYPE_HEAD v
-Proof
-  one_arg_tac
-QED
-
-Theorem dest_const_v_head:
-  do_opapp [dest_const_v; v] = SOME (env, exp) ∧
-  evaluate ^s env [exp] = (s', res) ⇒
-    ^safe_error_goal ∨
-    TERM_TYPE_HEAD v
-Proof
-  one_arg_tac
-QED
-
-Theorem dest_comb_v_head:
-  do_opapp [dest_comb_v; v] = SOME (env, exp) ∧
-  evaluate ^s env [exp] = (s', res) ⇒
-    ^safe_error_goal ∨
-    TERM_TYPE_HEAD v
-Proof
-  one_arg_tac
-QED
-
-Theorem dest_abs_v_head:
-  do_opapp [dest_abs_v; v] = SOME (env, exp) ∧
-  evaluate ^s env [exp] = (s', res) ⇒
-    ^safe_error_goal ∨
-    TERM_TYPE_HEAD v
-Proof
-  one_arg_tac
-QED
-
-Theorem dest_vartype_v_head:
-  do_opapp [dest_vartype_v; v] = SOME (env, exp) ∧
-  evaluate ^s env [exp] = (s', res) ⇒
-    ^safe_error_goal ∨
-    TYPE_TYPE_HEAD v
-Proof
-  one_arg_tac
-QED
-
-Theorem dest_type_v_head:
-  do_opapp [dest_type_v; v] = SOME (env, exp) ∧
-  evaluate ^s env [exp] = (s', res) ⇒
-    ^safe_error_goal ∨
-    TYPE_TYPE_HEAD v
-Proof
-  one_arg_tac
-QED
-
-Theorem dest_eq_v_head:
-  do_opapp [dest_eq_v; v] = SOME (env, exp) ∧
-  evaluate ^s env [exp] = (s', res) ⇒
-    ^safe_error_goal ∨
-    TERM_TYPE_HEAD v
-Proof
-  one_arg_tac
-QED
-
-Theorem call_tyvars_v_head:
-  do_opapp [call_tyvars_v; v] = SOME (env, exp) ∧
-  evaluate ^s env [exp] = (s', res) ⇒
-    ^safe_error_goal ∨
-    TYPE_TYPE_HEAD v
-Proof
-  one_arg_tac
-QED
-
-Theorem call_type_vars_in_term_v_head:
-  do_opapp [call_type_vars_in_term_v; v] = SOME (env, exp) ∧
-  evaluate ^s env [exp] = (s', res) ⇒
-    ^safe_error_goal ∨
-    TERM_TYPE_HEAD v
-Proof
-  one_arg_tac
-QED
-
-Theorem call_type_vars_in_term_v_head:
-  do_opapp [call_type_vars_in_term_v; v] = SOME (env, exp) ∧
-  evaluate ^s env [exp] = (s', res) ⇒
-    ^safe_error_goal ∨
-    TERM_TYPE_HEAD v
-Proof
-  one_arg_tac
-QED
-
-Theorem new_basic_definition_v_head:
-  do_opapp [new_basic_definition_v; v] = SOME (env, exp) ∧
-  evaluate ^s env [exp] = (s', res) ⇒
-    ^safe_error_goal ∨
-    TERM_TYPE_HEAD v
-Proof
-  one_arg_tac
-QED
-
-Theorem get_const_type_v_head:
-  do_opapp [get_const_type_v; v] = SOME (env, exp) ∧
-  evaluate ^s env [exp] = (s', res) ⇒
-    ^safe_error_goal ∨
-    STRING_TYPE_HEAD v
-Proof
-  one_arg_tac
-QED
-
-Theorem new_constant_v_head:
-  do_opapp [new_constant_v; v] = SOME (env, exp) ∧
-  evaluate ^s env [exp] = (s', res) ⇒
-    ^safe_error_goal ∨
-    PAIR_TYPE_HEAD STRING_TYPE_HEAD TYPE_TYPE_HEAD v
-Proof
-  one_arg_tac
-QED
-
-Theorem mk_var_v_head:
-  do_opapp [mk_var_v; v] = SOME (env, exp) ∧
-  evaluate ^s env [exp] = (s', res) ⇒
-    ^safe_error_goal ∨
-    PAIR_TYPE_HEAD STRING_TYPE_HEAD TYPE_TYPE_HEAD v
-Proof
-  one_arg_tac
-QED
-
-Theorem mk_comb_v_head:
-  do_opapp [mk_comb_v; v] = SOME (env, exp) ∧
-  evaluate ^s env [exp] = (s', res) ⇒
-    ^safe_error_goal ∨
-    PAIR_TYPE_HEAD TERM_TYPE_HEAD TERM_TYPE_HEAD v
-Proof
-  one_arg_tac
-QED
-
-Theorem get_type_arity_v_head:
-  do_opapp [get_type_arity_v; v] = SOME (env, exp) ∧
-  evaluate ^s env [exp] = (s', res) ⇒
-    ^safe_error_goal ∨
-    STRING_TYPE_HEAD v
-Proof
-  one_arg_tac
-QED
-
-Theorem mk_type_v_head:
-  do_opapp [mk_type_v; v] = SOME (env, exp) ∧
-  evaluate ^s env [exp] = (s', res) ⇒
-    ^safe_error_goal ∨
-    PAIR_TYPE_HEAD STRING_TYPE_HEAD (LIST_TYPE_HEAD TYPE_TYPE_HEAD) v
-Proof
-  one_arg_tac
-QED
-
-Theorem refl_v_head:
-  do_opapp [refl_v; v] = SOME (env, exp) ∧
-  evaluate ^s env [exp] = (s', res) ⇒
-    ^safe_error_goal ∨
-    TERM_TYPE_HEAD v
-Proof
-  one_arg_tac
-QED
-
-Theorem mk_const_v_head:
-  do_opapp [mk_const_v; v] = SOME (env, exp) ∧
-  evaluate ^s env [exp] = (s', res) ⇒
-    ^safe_error_goal ∨
-    PAIR_TYPE_HEAD STRING_TYPE_HEAD
-      (LIST_TYPE_HEAD (PAIR_TYPE_HEAD TYPE_TYPE_HEAD TYPE_TYPE_HEAD)) v
-Proof
-  one_arg_tac
-QED
-
-Theorem freesl_v_head:
-  do_opapp [freesl_v; v] = SOME (env, exp) ∧
-  evaluate ^s env [exp] = (s', res) ⇒
-    ^safe_error_goal ∨
-    LIST_TYPE_HEAD TERM_TYPE_HEAD v
-Proof
-  one_arg_tac
-QED
-
-Theorem assume_v_head:
-  do_opapp [assume_v; v] = SOME (env, exp) ∧
-  evaluate ^s env [exp] = (s', res) ⇒
-    ^safe_error_goal ∨
-    TERM_TYPE_HEAD v
-Proof
-  one_arg_tac
-QED
-
-Theorem hyp_v_head:
-  do_opapp [hyp_v; v] = SOME (env, exp) ∧
-  evaluate ^s env [exp] = (s', res) ⇒
-    ^safe_error_goal ∨
-    THM_TYPE_HEAD v
-Proof
-  one_arg_tac
-QED
-
-Theorem dest_thm_v_head:
-  do_opapp [dest_thm_v; v] = SOME (env, exp) ∧
-  evaluate ^s env [exp] = (s', res) ⇒
-    ^safe_error_goal ∨
-    THM_TYPE_HEAD v
-Proof
-  one_arg_tac
-QED
-
-Theorem mk_comb_1_v_head:
-  do_opapp [mk_comb_1_v; v] = SOME (env, exp) ∧
-  evaluate ^s env [exp] = (s', res) ⇒
-    ^safe_error_goal ∨
-    PAIR_TYPE_HEAD THM_TYPE_HEAD THM_TYPE_HEAD v
-Proof
-  one_arg_tac
-QED
-
-Theorem new_basic_type_definition_v_head:
-  do_opapp [new_basic_type_definition_v; v] = SOME (env, exp) ∧
-  evaluate ^s env [exp] = (s', res) ⇒
-    ^safe_error_goal ∨
-    (PAIR_TYPE_HEAD STRING_TYPE_HEAD $
-       PAIR_TYPE_HEAD STRING_TYPE_HEAD $
-          PAIR_TYPE_HEAD STRING_TYPE_HEAD THM_TYPE_HEAD) v
-Proof
-  one_arg_tac
-QED
-
-Theorem call_type_subst_v_head:
-  do_partial_app call_type_subst_v v = SOME g ∧
+Theorem call_variant_v_head:
+  do_partial_app call_variant_v v = SOME g ∧
   do_opapp [g; w] = SOME (env, exp) ∧
   evaluate ^s env [exp] = (s', res) ⇒
     ^safe_error_goal ∨
-    LIST_TYPE_HEAD (PAIR_TYPE_HEAD TYPE_TYPE_HEAD TYPE_TYPE_HEAD) v ∧
-    TYPE_TYPE_HEAD w
+    LIST_TYPE_HEAD TERM_TYPE_HEAD v ∧
+    TERM_TYPE_HEAD w
 Proof
-  one_arg_tac
+  prove_head_tac
 QED
 
 Theorem vsubst_v_head:
@@ -1444,7 +1072,338 @@ Theorem vsubst_v_head:
     LIST_TYPE_HEAD (PAIR_TYPE_HEAD TERM_TYPE_HEAD TERM_TYPE_HEAD) v ∧
     TERM_TYPE_HEAD w
 Proof
-  one_arg_tac
+  prove_head_tac
+QED
+
+Theorem dest_type_v_head:
+  do_opapp [dest_type_v; v] = SOME (env, exp) ∧
+  evaluate ^s env [exp] = (s', res) ⇒
+    ^safe_error_goal ∨
+    TYPE_TYPE_HEAD v
+Proof
+  prove_head_tac
+QED
+
+Theorem is_type_v_head:
+  do_opapp [is_type_v; v] = SOME (env, exp) ∧
+  evaluate ^s env [exp] = (s', res) ⇒
+    ^safe_error_goal ∨
+    TYPE_TYPE_HEAD v
+Proof
+  prove_head_tac
+QED
+
+Theorem is_vartype_v_head:
+  do_opapp [is_vartype_v; v] = SOME (env, exp) ∧
+  evaluate ^s env [exp] = (s', res) ⇒
+    ^safe_error_goal ∨
+    TYPE_TYPE_HEAD v
+Proof
+  prove_head_tac
+QED
+
+Theorem is_var_v_head:
+  do_opapp [is_var_v; v] = SOME (env, exp) ∧
+  evaluate ^s env [exp] = (s', res) ⇒
+    ^safe_error_goal ∨
+    TERM_TYPE_HEAD v
+Proof
+  prove_head_tac
+QED
+
+Theorem is_const_v_head:
+  do_opapp [is_const_v; v] = SOME (env, exp) ∧
+  evaluate ^s env [exp] = (s', res) ⇒
+    ^safe_error_goal ∨
+    TERM_TYPE_HEAD v
+Proof
+  prove_head_tac
+QED
+
+Theorem is_abs_v_head:
+  do_opapp [is_abs_v; v] = SOME (env, exp) ∧
+  evaluate ^s env [exp] = (s', res) ⇒
+    ^safe_error_goal ∨
+    TERM_TYPE_HEAD v
+Proof
+  prove_head_tac
+QED
+
+Theorem is_comb_v_head:
+  do_opapp [is_comb_v; v] = SOME (env, exp) ∧
+  evaluate ^s env [exp] = (s', res) ⇒
+    ^safe_error_goal ∨
+    TERM_TYPE_HEAD v
+Proof
+  prove_head_tac
+QED
+
+Theorem rand_v_head:
+  do_opapp [rand_v; v] = SOME (env, exp) ∧
+  evaluate ^s env [exp] = (s', res) ⇒
+    ^safe_error_goal ∨
+    TERM_TYPE_HEAD v
+Proof
+  prove_head_tac
+QED
+
+Theorem rator_v_head:
+  do_opapp [rator_v; v] = SOME (env, exp) ∧
+  evaluate ^s env [exp] = (s', res) ⇒
+    ^safe_error_goal ∨
+    TERM_TYPE_HEAD v
+Proof
+  prove_head_tac
+QED
+
+Theorem dest_var_v_head:
+  do_opapp [dest_var_v; v] = SOME (env, exp) ∧
+  evaluate ^s env [exp] = (s', res) ⇒
+    ^safe_error_goal ∨
+    TERM_TYPE_HEAD v
+Proof
+  prove_head_tac
+QED
+
+Theorem dest_const_v_head:
+  do_opapp [dest_const_v; v] = SOME (env, exp) ∧
+  evaluate ^s env [exp] = (s', res) ⇒
+    ^safe_error_goal ∨
+    TERM_TYPE_HEAD v
+Proof
+  prove_head_tac
+QED
+
+Theorem dest_comb_v_head:
+  do_opapp [dest_comb_v; v] = SOME (env, exp) ∧
+  evaluate ^s env [exp] = (s', res) ⇒
+    ^safe_error_goal ∨
+    TERM_TYPE_HEAD v
+Proof
+  prove_head_tac
+QED
+
+Theorem dest_abs_v_head:
+  do_opapp [dest_abs_v; v] = SOME (env, exp) ∧
+  evaluate ^s env [exp] = (s', res) ⇒
+    ^safe_error_goal ∨
+    TERM_TYPE_HEAD v
+Proof
+  prove_head_tac
+QED
+
+Theorem dest_vartype_v_head:
+  do_opapp [dest_vartype_v; v] = SOME (env, exp) ∧
+  evaluate ^s env [exp] = (s', res) ⇒
+    ^safe_error_goal ∨
+    TYPE_TYPE_HEAD v
+Proof
+  prove_head_tac
+QED
+
+Theorem dest_type_v_head:
+  do_opapp [dest_type_v; v] = SOME (env, exp) ∧
+  evaluate ^s env [exp] = (s', res) ⇒
+    ^safe_error_goal ∨
+    TYPE_TYPE_HEAD v
+Proof
+  prove_head_tac
+QED
+
+Theorem dest_eq_v_head:
+  do_opapp [dest_eq_v; v] = SOME (env, exp) ∧
+  evaluate ^s env [exp] = (s', res) ⇒
+    ^safe_error_goal ∨
+    TERM_TYPE_HEAD v
+Proof
+  prove_head_tac
+QED
+
+Theorem call_tyvars_v_head:
+  do_opapp [call_tyvars_v; v] = SOME (env, exp) ∧
+  evaluate ^s env [exp] = (s', res) ⇒
+    ^safe_error_goal ∨
+    TYPE_TYPE_HEAD v
+Proof
+  prove_head_tac
+QED
+
+Theorem call_type_vars_in_term_v_head:
+  do_opapp [call_type_vars_in_term_v; v] = SOME (env, exp) ∧
+  evaluate ^s env [exp] = (s', res) ⇒
+    ^safe_error_goal ∨
+    TERM_TYPE_HEAD v
+Proof
+  prove_head_tac
+QED
+
+Theorem call_type_vars_in_term_v_head:
+  do_opapp [call_type_vars_in_term_v; v] = SOME (env, exp) ∧
+  evaluate ^s env [exp] = (s', res) ⇒
+    ^safe_error_goal ∨
+    TERM_TYPE_HEAD v
+Proof
+  prove_head_tac
+QED
+
+Theorem new_basic_definition_v_head:
+  do_opapp [new_basic_definition_v; v] = SOME (env, exp) ∧
+  evaluate ^s env [exp] = (s', res) ⇒
+    ^safe_error_goal ∨
+    TERM_TYPE_HEAD v
+Proof
+  prove_head_tac
+QED
+
+Theorem get_const_type_v_head:
+  do_opapp [get_const_type_v; v] = SOME (env, exp) ∧
+  evaluate ^s env [exp] = (s', res) ⇒
+    ^safe_error_goal ∨
+    STRING_TYPE_HEAD v
+Proof
+  prove_head_tac
+QED
+
+Theorem new_constant_v_head:
+  do_opapp [new_constant_v; v] = SOME (env, exp) ∧
+  evaluate ^s env [exp] = (s', res) ⇒
+    ^safe_error_goal ∨
+    PAIR_TYPE_HEAD STRING_TYPE_HEAD TYPE_TYPE_HEAD v
+Proof
+  prove_head_tac
+QED
+
+Theorem mk_var_v_head:
+  do_opapp [mk_var_v; v] = SOME (env, exp) ∧
+  evaluate ^s env [exp] = (s', res) ⇒
+    ^safe_error_goal ∨
+    PAIR_TYPE_HEAD STRING_TYPE_HEAD TYPE_TYPE_HEAD v
+Proof
+  prove_head_tac
+QED
+
+Theorem mk_comb_v_head:
+  do_opapp [mk_comb_v; v] = SOME (env, exp) ∧
+  evaluate ^s env [exp] = (s', res) ⇒
+    ^safe_error_goal ∨
+    PAIR_TYPE_HEAD TERM_TYPE_HEAD TERM_TYPE_HEAD v
+Proof
+  prove_head_tac
+QED
+
+Theorem get_type_arity_v_head:
+  do_opapp [get_type_arity_v; v] = SOME (env, exp) ∧
+  evaluate ^s env [exp] = (s', res) ⇒
+    ^safe_error_goal ∨
+    STRING_TYPE_HEAD v
+Proof
+  prove_head_tac
+QED
+
+Theorem mk_type_v_head:
+  do_opapp [mk_type_v; v] = SOME (env, exp) ∧
+  evaluate ^s env [exp] = (s', res) ⇒
+    ^safe_error_goal ∨
+    PAIR_TYPE_HEAD STRING_TYPE_HEAD (LIST_TYPE_HEAD TYPE_TYPE_HEAD) v
+Proof
+  prove_head_tac
+QED
+
+Theorem refl_v_head:
+  do_opapp [refl_v; v] = SOME (env, exp) ∧
+  evaluate ^s env [exp] = (s', res) ⇒
+    ^safe_error_goal ∨
+    TERM_TYPE_HEAD v
+Proof
+  prove_head_tac
+QED
+
+Theorem mk_const_v_head:
+  do_opapp [mk_const_v; v] = SOME (env, exp) ∧
+  evaluate ^s env [exp] = (s', res) ⇒
+    ^safe_error_goal ∨
+    PAIR_TYPE_HEAD STRING_TYPE_HEAD
+      (LIST_TYPE_HEAD (PAIR_TYPE_HEAD TYPE_TYPE_HEAD TYPE_TYPE_HEAD)) v
+Proof
+  prove_head_tac
+QED
+
+Theorem freesl_v_head:
+  do_opapp [freesl_v; v] = SOME (env, exp) ∧
+  evaluate ^s env [exp] = (s', res) ⇒
+    ^safe_error_goal ∨
+    LIST_TYPE_HEAD TERM_TYPE_HEAD v
+Proof
+  prove_head_tac
+QED
+
+Theorem assume_v_head:
+  do_opapp [assume_v; v] = SOME (env, exp) ∧
+  evaluate ^s env [exp] = (s', res) ⇒
+    ^safe_error_goal ∨
+    TERM_TYPE_HEAD v
+Proof
+  prove_head_tac
+QED
+
+Theorem hyp_v_head:
+  do_opapp [hyp_v; v] = SOME (env, exp) ∧
+  evaluate ^s env [exp] = (s', res) ⇒
+    ^safe_error_goal ∨
+    THM_TYPE_HEAD v
+Proof
+  prove_head_tac
+QED
+
+Theorem dest_thm_v_head:
+  do_opapp [dest_thm_v; v] = SOME (env, exp) ∧
+  evaluate ^s env [exp] = (s', res) ⇒
+    ^safe_error_goal ∨
+    THM_TYPE_HEAD v
+Proof
+  prove_head_tac
+QED
+
+Theorem mk_comb_1_v_head:
+  do_opapp [mk_comb_1_v; v] = SOME (env, exp) ∧
+  evaluate ^s env [exp] = (s', res) ⇒
+    ^safe_error_goal ∨
+    PAIR_TYPE_HEAD THM_TYPE_HEAD THM_TYPE_HEAD v
+Proof
+  prove_head_tac
+QED
+
+Theorem new_basic_type_definition_v_head:
+  do_opapp [new_basic_type_definition_v; v] = SOME (env, exp) ∧
+  evaluate ^s env [exp] = (s', res) ⇒
+    ^safe_error_goal ∨
+    (PAIR_TYPE_HEAD STRING_TYPE_HEAD $
+       PAIR_TYPE_HEAD STRING_TYPE_HEAD $
+          PAIR_TYPE_HEAD STRING_TYPE_HEAD THM_TYPE_HEAD) v
+Proof
+  prove_head_tac
+QED
+
+Theorem call_type_subst_v_head:
+  do_partial_app call_type_subst_v v = SOME g ∧
+  do_opapp [g; w] = SOME (env, exp) ∧
+  evaluate ^s env [exp] = (s', res) ⇒
+    ^safe_error_goal ∨
+    LIST_TYPE_HEAD (PAIR_TYPE_HEAD TYPE_TYPE_HEAD TYPE_TYPE_HEAD) v ∧
+    TYPE_TYPE_HEAD w
+Proof
+  prove_head_tac
+QED
+
+Theorem vsubst_v_head:
+  do_partial_app vsubst_v v = SOME g ∧
+  do_opapp [g; w] = SOME (env, exp) ∧
+  evaluate ^s env [exp] = (s', res) ⇒
+    ^safe_error_goal ∨
+    LIST_TYPE_HEAD (PAIR_TYPE_HEAD TERM_TYPE_HEAD TERM_TYPE_HEAD) v ∧
+    TERM_TYPE_HEAD w
+Proof
+  prove_head_tac
 QED
 
 Theorem inst_v_head:
@@ -1455,7 +1414,7 @@ Theorem inst_v_head:
     LIST_TYPE_HEAD (PAIR_TYPE_HEAD TYPE_TYPE_HEAD TYPE_TYPE_HEAD) v ∧
     TERM_TYPE_HEAD w
 Proof
-  one_arg_tac
+  prove_head_tac
 QED
 
 Theorem abs_1_v_head:
@@ -1466,7 +1425,7 @@ Theorem abs_1_v_head:
     THM_TYPE_HEAD w ∧
     TERM_TYPE_HEAD v
 Proof
-  one_arg_tac
+  prove_head_tac
 QED
 
 Theorem eq_mp_v_head:
@@ -1477,7 +1436,7 @@ Theorem eq_mp_v_head:
     THM_TYPE_HEAD v ∧
     THM_TYPE_HEAD w
 Proof
-  one_arg_tac
+  prove_head_tac
 QED
 
 Theorem deduct_antisym_rule_v_head:
@@ -1488,7 +1447,7 @@ Theorem deduct_antisym_rule_v_head:
     THM_TYPE_HEAD v ∧
     THM_TYPE_HEAD w
 Proof
-  one_arg_tac
+  prove_head_tac
 QED
 
 Theorem inst_type_v_head:
@@ -1499,7 +1458,7 @@ Theorem inst_type_v_head:
     THM_TYPE_HEAD w ∧
     LIST_TYPE_HEAD (PAIR_TYPE_HEAD TYPE_TYPE_HEAD TYPE_TYPE_HEAD) v
 Proof
-  one_arg_tac
+  prove_head_tac
 QED
 
 Theorem inst_1_v_head:
@@ -1510,7 +1469,7 @@ Theorem inst_1_v_head:
     THM_TYPE_HEAD w ∧
     LIST_TYPE_HEAD (PAIR_TYPE_HEAD TERM_TYPE_HEAD TERM_TYPE_HEAD) v
 Proof
-  one_arg_tac
+  prove_head_tac
 QED
 
 Theorem new_axiom_v_head:
@@ -1519,7 +1478,7 @@ Theorem new_axiom_v_head:
     ^safe_error_goal ∨
     TERM_TYPE_HEAD v
 Proof
-  one_arg_tac
+  prove_head_tac
 QED
 
 Theorem call_type_of_v_head:
@@ -1528,7 +1487,7 @@ Theorem call_type_of_v_head:
     ^safe_error_goal ∨
     TERM_TYPE_HEAD v
 Proof
-  one_arg_tac
+  prove_head_tac
 QED
 
 Theorem call_vfree_in_v_head:
@@ -1538,7 +1497,7 @@ Theorem call_vfree_in_v_head:
     ^safe_error_goal ∨
     TERM_TYPE_HEAD v
 Proof
-  one_arg_tac
+  prove_head_tac
 QED
 
 Theorem call_freesin_v_head:
@@ -1549,7 +1508,7 @@ Theorem call_freesin_v_head:
     LIST_TYPE_HEAD TERM_TYPE_HEAD v ∧
     TERM_TYPE_HEAD w
 Proof
-  one_arg_tac
+  prove_head_tac
 QED
 
 Theorem mk_abs_v_head:
@@ -1558,7 +1517,7 @@ Theorem mk_abs_v_head:
     ^safe_error_goal ∨
     PAIR_TYPE_HEAD TERM_TYPE_HEAD TERM_TYPE_HEAD v
 Proof
-  one_arg_tac
+  prove_head_tac
 QED
 
 Theorem call_frees_v_head:
@@ -1567,18 +1526,20 @@ Theorem call_frees_v_head:
     ^safe_error_goal ∨
     TERM_TYPE_HEAD v
 Proof
-  one_arg_tac
+  prove_head_tac
 QED
 
-(*
+Theorem inst_v_head:
+  do_partial_app inst_v v = SOME g ∧
+  do_opapp [g; w] = SOME (env, exp) ∧
+  evaluate ^s env [exp] = (s', res) ⇒
+    ^safe_error_goal ∨
+    LIST_TYPE_HEAD (PAIR_TYPE_HEAD TYPE_TYPE_HEAD TYPE_TYPE_HEAD) v ∧
+    TERM_TYPE_HEAD w
+Proof
+  prove_head_tac
+QED
 
-Note: these head theorems should be proved as much as possible using
-only drule with generic lemmas like evaluate_ty_check,
-evaluate_tm_check etc.
-
-  new_type_v_thm
-
-*)
 
 (* -------------------------------------------------------------------------
  * Misc. simps
